prove FUpd_open

src/logic/FancyUpdate.v
@@ -19,8 +19,32 @@ Section PCM_OWN.
   Definition OwnE `{@GRA.inG CoPset.t Σ} (E : coPset) := OwnM (Some E).
   Definition OwnD `{@GRA.inG Gset.t Σ} (D : gset positive) := OwnM (Some D).
   Definition inv `{Interp} `{@GRA.inG (Auth.t (positive ==> URA.agree Var)%ra) Σ}
-    (n : positive) (x : Var) :=
-    OwnM (Auth.white (@maps_to_res positive (URA.agree Var) n (Some (Some x)))).
+    (i : positive) (x : Var) :=
+    OwnM (Auth.white (@maps_to_res positive (URA.agree Var) i (Some (Some x)))).
+
+  Lemma OwnE_disjoint `{@GRA.inG CoPset.t Σ} (E1 E2 : coPset) :
+    E1 ## E2 -> OwnE (E1 ∪ E2) ⊣⊢ OwnE E1 ∗ OwnE E2.
+  Proof.
+    i. unfold OwnE. iSplit.
+    - iApply into_sep. eapply into_sep_ownM.
+      unfold IsOp, URA.add. unseal "ra". ss. des_ifs.
+    - iApply from_sep. eapply from_sep_ownM.
+      unfold IsOp, URA.add. unseal "ra". ss. des_ifs.
+  Qed.
+
+  Lemma OwnE_not_disjoint `{@GRA.inG CoPset.t Σ} (E1 E2 : coPset) :
+    ¬ E1 ## E2 -> OwnE E1 ∗ OwnE E2 ⊢ False.
+  Proof.
+    i. iIntros "H". iAssert (OwnM (None : CoPset.t)) with "[H]" as "H".
+    - iRevert "H". iApply from_sep. eapply from_sep_ownM.
+      unfold IsOp. unfold URA.add. unseal "ra". ss. des_ifs.
+    - iPoseProof (OwnM_valid with "H") as "H".
+      iRevert "H". iPureIntro. unfold URA.wf. unseal "ra". ss.
+  Qed.
+
+  Global Instance inv_persistent `{Interp} `{@GRA.inG (Auth.t (positive ==> URA.agree Var)%ra) Σ}
+    i p : Persistent (inv i p).
+  Admitted.
 
 End PCM_OWN.
 
@@ -35,16 +59,29 @@ Section WORLD_SATISFACTION.
   Definition inv_auth (I : gmap positive Var) :=
     OwnM (@Auth.black
             (positive ==> URA.agree Var)%ra
-            (fun (i : positive) =>
-               match I !! i return (URA.agree Var) with
-               | Some x => Some (Some x)
-               | None => None
-               end)).
+            (fun (i : positive) => Some <$> (I !! i))).
 
   Definition inv_satall (I : gmap positive Var) :=
-    ([∗ map] i ↦ x ∈ I, prop x ∗ OwnD {[i]} ∨ OwnE {[i]})%I.
+    ([∗ map] i ↦ p ∈ I, prop p ∗ OwnD {[i]} ∨ OwnE {[i]})%I.
 
   Definition wsat : iProp := (∃ I, inv_auth I ∗ inv_satall I)%I.
+
+  Lemma wsat_inv_alloc p :
+    wsat ∗ prop p ⊢ |==> ∃ i, inv i p ∗ wsat.
+  Admitted.
+
+  Lemma wsat_inv_open i p :
+    inv i p ∗ wsat ∗ OwnE {[i]} ⊢ |==> prop p ∗ wsat ∗ OwnD {[i]}.
+  Proof.
+    iIntros "(I & [% [AUTH SAT]] & EN)".
+    unfold inv, inv_auth, inv_satall.
+    Search Auth.white.
+    Search OwnM.
+  Admitted.
+
+  Lemma wsat_inv_close i p :
+    inv i p ∗ wsat ∗ prop p ∗ OwnD {[i]} ⊢ |==> wsat ∗ OwnE {[i]}.
+  Admitted.
 
 End WORLD_SATISFACTION.
 
@@ -58,5 +95,28 @@ Section FANCY_UPDATE.
 
   Definition FUpd (E1 E2 : coPset) (P : iProp) : iProp :=
     wsat ∗ OwnE E1 -∗ #=> (wsat ∗ OwnE E2 ∗ P).
+
+  Lemma FUpd_open E i p (IN : i ∈ E) :
+    inv i p ⊢ FUpd E (E∖{[i]}) (prop p ∗ (prop p -∗ FUpd (E∖{[i]}) E True)).
+  Proof.
+    iIntros "#H [WSAT EN]".
+    iAssert (OwnE (E ∖ {[i]}) ∗ OwnE {[i]})%I with "[EN]" as "[EN1 EN2]".
+    { iApply OwnE_disjoint. { set_solver. }
+      iRevert "EN". replace E with ((E ∖ {[i]}) ∪ {[i]}) at 1. eauto.
+      eapply leibniz_equiv. symmetry. transitivity ({[i]} ∪ E ∖ {[i]}).
+      - apply union_difference; set_solver.
+      - eapply union_comm.
+    }
+    iMod (wsat_inv_open i p with "[H WSAT EN2]") as "(P & WSAT & DIS)". { iFrame. iApply "H". }
+    iModIntro. iFrame. iIntros "P [WSAT EN1]".
+    iMod (wsat_inv_close i p with "[H WSAT P  DIS]") as "(WSAT & EN2)". { iFrame. iApply "H". }
+    iModIntro. iFrame. iSplit; eauto.
+    iAssert (OwnE (E∖{[i]} ∪ {[i]}))%I with "[EN1 EN2]" as "EN".
+    { iApply OwnE_disjoint. set_solver. iFrame. }
+    replace (E ∖ {[i]} ∪ {[i]}) with E. eauto.
+    eapply leibniz_equiv. transitivity ({[i]} ∪ E ∖ {[i]}).
+    - apply union_difference; set_solver.
+    - eapply union_comm.
+  Qed.
 
 End FANCY_UPDATE.
